tests/bug-reports/Bug2172.fst
@@ -1,12 +1,14 @@
 module Bug2172
-
+#push-options "--ext context_pruning"
 // one existential quantification over two variables (`p2` below) is
 // different from two extistential quantifications over one variable
 // each (`p1` below)
-
 let p1 = exists (x: int). exists (y: int). 0 == x + y
 let p2 = exists (x: int)         (y: int). 0 == x + y
 
-let _ = assert p1
-let _ = assert p2
+let test0 (witness:nat) = assert p1
+#pop-options
+#push-options "--ext 'context_pruning='"
+let test1 = assert p2
+#pop-options
 let _ = assert (p1 <==> p2)
